QVM/MathSpec.v
@@ -1,0 +1,965 @@
+Require Import Coq.btauto.Btauto Coq.NArith.Nnat Bool. 
+Require Import Dirac.
+Require Import BasicUtility.
+Local Open Scope nat_scope.
+
+(* Here we defined the specification of carry value for each bit. *)
+(* fb_push is to take a qubit and then push it to the zero position 
+        in the bool function representation of a number. *)
+Lemma mod_sum_lt :
+  forall x y M,
+    x < M ->
+    y < M ->
+    (x + y) mod M < x <-> x + y >= M.
+Proof.
+  intros. split; intros.
+  - assert ((x + y) mod M < x + y) by lia.
+    rewrite Nat.div_mod with (y := M) in H2 by lia.
+    assert (0 < (x + y) / M) by nia.
+    rewrite Nat.div_str_pos_iff in H3 by lia. lia.
+  - rewrite Nat.mod_eq by lia.
+    assert (1 <= (x + y) / M < 2).
+    { split.
+      apply Nat.div_le_lower_bound; lia.
+      apply Nat.div_lt_upper_bound; lia.
+    }
+    replace (M * ((x + y) / M)) with M by nia.
+    lia.
+Qed.
+
+
+Lemma mod_sum_lt_bool :
+  forall x y M,
+    x < M ->
+    y < M ->
+    ¬ (M <=? x + y) = (x <=? (x + y) mod M).
+Proof.
+  intros. bdestruct (M <=? x + y); bdestruct (x <=? (x + y) mod M); try easy.
+  assert ((x + y) mod M < x) by (apply mod_sum_lt; lia). lia.
+  assert (x + y >= M) by (apply mod_sum_lt; lia). lia.
+Qed.
+
+
+Definition allfalse := fun (_:nat) => false.
+
+Definition majb a b c := (a && b) ⊕ (b && c) ⊕ (a && c).
+
+Definition fb_push b f : nat -> bool :=
+  fun x => match x with
+        | O => b
+        | S n => f n
+        end.
+
+Lemma fb_push_right:
+  forall n b f, 0 < n -> fb_push b f n = f (n-1).
+Proof.
+  intros. induction n. lia.
+  simpl. assert ((n - 0) = n) by lia.
+  rewrite H0. reflexivity.
+Qed.
+
+Lemma fb_push_same : forall b f g, (forall i, fb_push b f i = fb_push b g i) -> f = g.
+Proof.
+intros.
+apply functional_extensionality; intros.
+specialize (H (S x)).
+rewrite fb_push_right in H; try lia.
+rewrite fb_push_right in H; try lia.
+simpl in H.
+assert (x-0 = x) by lia. rewrite H0 in H. easy. 
+Qed.
+
+(* fb_push_n is the n repeatation of fb_push.
+Definition fb_push_n n f g : nat -> bool :=
+  fun i => if (i <? n) then f i else g (i - n).
+*)
+
+(* A function to compile positive to a bool function. *)
+Fixpoint pos2fb p : nat -> bool :=
+  match p with
+  | xH => fb_push true allfalse
+  | xI p' => fb_push true (pos2fb p')
+  | xO p' => fb_push false (pos2fb p')
+  end.
+
+(* A function to compile N to a bool function. *)
+Definition N2fb n : nat -> bool :=
+  match n with
+  | 0%N => allfalse
+  | Npos p => pos2fb p
+  end.
+
+Definition nat2fb n := N2fb (N.of_nat n).
+
+Definition add_c b x y :=
+  match b with
+  | false => Pos.add x y
+  | true => Pos.add_carry x y
+  end.
+
+Fixpoint carry b n f g :=
+  match n with
+  | 0 => b
+  | S n' => let c := carry b n' f g in
+           let a := f n' in
+           let b := g n' in
+           (a && b) ⊕ (b && c) ⊕ (a && c)
+  end.
+
+Lemma carry_1 : forall b f g, carry b 1 f g = majb (f 0) (g 0) b.
+Proof.
+ intros. simpl. unfold majb. easy.
+Qed.
+
+Lemma carry_n : forall n b f g, carry b (S n) f g = majb (f n) (g n) (carry b n f g).
+Proof.
+ intros. simpl. unfold majb. easy.
+Qed.
+
+Lemma carry_sym :
+  forall b n f g,
+    carry b n f g = carry b n g f.
+Proof.
+  intros. induction n. reflexivity.
+  simpl. rewrite IHn. btauto.
+Qed.
+
+Lemma carry_false_0_l: forall n f, 
+    carry false n allfalse f = false.
+Proof.
+  unfold allfalse.
+  induction n.
+  simpl.
+  reflexivity.
+  intros. simpl.
+  rewrite IHn. rewrite andb_false_r.
+  reflexivity.
+Qed.
+
+Lemma carry_false_0_r: forall n f, 
+    carry false n f allfalse = false.
+Proof.
+  unfold allfalse.
+  induction n.
+  simpl.
+  reflexivity.
+  intros. simpl.
+  rewrite IHn. rewrite andb_false_r.
+  reflexivity.
+Qed.
+
+Lemma carry_fbpush :
+  forall n a ax ay fx fy,
+    carry a (S n) (fb_push ax fx) (fb_push ay fy) = carry (majb a ax ay) n fx fy.
+Proof.
+  induction n; intros.
+  simpl. unfold majb. btauto.
+  remember (S n) as Sn. simpl. rewrite IHn. unfold fb_push. subst.
+  simpl. easy.
+Qed.
+
+Lemma carry_succ :
+  forall m p,
+    carry true m (pos2fb p) allfalse = pos2fb (Pos.succ p) m ⊕ (pos2fb p) m.
+Proof.
+  induction m; intros. simpl. destruct p; reflexivity.
+  replace allfalse with (fb_push false allfalse).
+  2:{ unfold fb_push, allfalse. apply functional_extensionality. intros. destruct x; reflexivity.
+  }
+  Local Opaque fb_push carry.
+  destruct p; simpl.
+  rewrite carry_fbpush; unfold majb; simpl. rewrite IHm. reflexivity.
+  rewrite carry_fbpush; unfold majb; simpl. rewrite carry_false_0_r. Local Transparent fb_push. simpl. btauto.
+  rewrite carry_fbpush; unfold majb; simpl. Local Transparent carry. destruct m; reflexivity.
+Qed.
+
+Lemma carry_succ' :
+  forall m p,
+    carry true m allfalse (pos2fb p) = pos2fb (Pos.succ p) m ⊕ (pos2fb p) m.
+Proof.
+  intros. rewrite carry_sym. apply carry_succ.
+Qed.
+
+Lemma carry_succ0 :
+  forall m, carry true m allfalse allfalse = pos2fb xH m.
+Proof.
+  induction m. easy. 
+  replace allfalse with (fb_push false allfalse).
+  2:{ unfold fb_push, allfalse. apply functional_extensionality. intros. destruct x; reflexivity.
+  }
+  rewrite carry_fbpush. unfold majb. simpl. rewrite carry_false_0_l. easy.
+Qed.
+
+Lemma carry_add_pos_eq :
+  forall m b p q,
+    carry b m (pos2fb p) (pos2fb q) ⊕ (pos2fb p) m ⊕ (pos2fb q) m = pos2fb (add_c b p q) m.
+Proof.
+  induction m; intros. simpl. destruct p, q, b; reflexivity.
+  Local Opaque carry.
+  destruct p, q, b; simpl; rewrite carry_fbpush; 
+    try (rewrite IHm; reflexivity);
+    try (unfold majb; simpl; 
+         try rewrite carry_succ; try rewrite carry_succ'; 
+         try rewrite carry_succ0; try rewrite carry_false_0_l;
+         try rewrite carry_false_0_r;
+         unfold allfalse; try btauto; try (destruct m; reflexivity)).
+Qed.
+
+Lemma carry_add_eq_carry0 :
+  forall m x y,
+    carry false m (N2fb x) (N2fb y) ⊕ (N2fb x) m ⊕ (N2fb y) m = (N2fb (x + y)) m.
+Proof.
+  intros.
+  destruct x as [|p]; destruct y as [|q]; simpl; unfold allfalse.
+  rewrite carry_false_0_l. easy.
+  rewrite carry_false_0_l. btauto.
+  rewrite carry_false_0_r. btauto.
+  apply carry_add_pos_eq.
+Qed.
+
+Lemma carry_add_eq_carry1 :
+  forall m x y,
+    carry true m (N2fb x) (N2fb y) ⊕ (N2fb x) m ⊕ (N2fb y) m = (N2fb (x + y + 1)) m.
+Proof.
+  intros. 
+  destruct x as [|p]; destruct y as [|q]; simpl; unfold allfalse.
+  rewrite carry_succ0. destruct m; easy.
+  rewrite carry_succ'. replace (q + 1)%positive with (Pos.succ q) by lia. btauto.
+  rewrite carry_succ. replace (p + 1)%positive with (Pos.succ p) by lia. btauto.
+  rewrite carry_add_pos_eq. unfold add_c. rewrite Pos.add_carry_spec.
+  replace (p + q + 1)%positive with (Pos.succ (p + q)) by lia. easy.
+Qed.
+
+Definition fbxor f g := fun (i : nat) => f i ⊕ g i.
+
+Definition msma i b f g := fun (x : nat) => if (x <? i) then 
+        (carry b (S x) f g ⊕ (f (S x))) else (if (x =? i) then carry b (S x) f g else f x).
+
+Definition msmb i (b : bool) f g := fun (x : nat) => if (x <=? i) then (f x ⊕ g x) else g x.
+
+Definition msmc i b f g := fun (x : nat) => if (x <=? i) then (f x ⊕ g x) else (carry b x f g ⊕ f x ⊕ g x).
+
+Definition sumfb b f g := fun (x : nat) => carry b x f g ⊕ f x ⊕ g x.
+
+Definition negatem i (f : nat -> bool) := fun (x : nat) => if (x <? i) then ¬ (f x) else f x.
+
+Lemma sumfb_correct_carry0 :
+  forall x y,
+    sumfb false (nat2fb x) (nat2fb y) = nat2fb (x + y).
+Proof.
+  intros. unfold nat2fb. rewrite Nnat.Nat2N.inj_add.
+  apply functional_extensionality. intros. unfold sumfb. rewrite carry_add_eq_carry0. easy.
+Qed.
+
+Lemma sumfb_correct_carry1 :
+  forall x y,
+    sumfb true (nat2fb x) (nat2fb y) = nat2fb (x + y + 1).
+Proof.
+  intros. unfold nat2fb. do 2 rewrite Nnat.Nat2N.inj_add.
+  apply functional_extensionality. intros. unfold sumfb. rewrite carry_add_eq_carry1. easy.
+Qed.
+
+Lemma sumfb_correct_N_carry0 :
+  forall x y,
+    sumfb false (N2fb x) (N2fb y) = N2fb (x + y).
+Proof.
+  intros. apply functional_extensionality. intros. unfold sumfb. rewrite carry_add_eq_carry0. easy.
+Qed.
+
+Lemma pos2fb_Postestbit :
+  forall n i,
+    (pos2fb n) i = Pos.testbit n (N.of_nat i).
+Proof.
+  induction n; intros.
+  - destruct i; simpl. easy. rewrite IHn. destruct i; simpl. easy. rewrite Pos.pred_N_succ. easy.
+  - destruct i; simpl. easy. rewrite IHn. destruct i; simpl. easy. rewrite Pos.pred_N_succ. easy.
+  - destruct i; simpl. easy. easy.
+Qed.
+
+Lemma N2fb_Ntestbit :
+  forall n i,
+    (N2fb n) i = N.testbit n (N.of_nat i).
+Proof.
+  intros. destruct n. easy.
+  simpl. apply pos2fb_Postestbit.
+Qed.
+
+Lemma Z2N_Nat2Z_Nat2N :
+  forall x,
+    Z.to_N (Z.of_nat x) = N.of_nat x.
+Proof.
+  destruct x; easy.
+Qed.
+
+Lemma Nofnat_mod :
+  forall x y,
+    y <> 0 ->
+    N.of_nat (x mod y) = ((N.of_nat x) mod (N.of_nat y))%N.
+Proof.
+  intros. specialize (Zdiv.mod_Zmod x y H) as G.
+  repeat rewrite <- Z2N_Nat2Z_Nat2N. rewrite G. rewrite Z2N.inj_mod; lia.
+Qed.
+
+Lemma Nofnat_pow :
+  forall x y,
+    N.of_nat (x ^ y) = ((N.of_nat x) ^ (N.of_nat y))%N.
+Proof.
+  intros. induction y. easy.
+  Local Opaque N.pow. replace (N.of_nat (S y)) with ((N.of_nat y) + 1)%N by lia.
+ simpl. rewrite N.pow_add_r. rewrite N.pow_1_r. rewrite Nnat.Nat2N.inj_mul. rewrite IHy. lia.
+Qed.
+
+Lemma Ntestbit_lt_pow2n :
+  forall x n,
+    (x < 2^n)%N ->
+    N.testbit x n = false.
+Proof.
+  intros. apply N.mod_small in H. rewrite <- H. apply N.mod_pow2_bits_high. lia.
+Qed.
+
+Lemma Ntestbit_in_pow2n_pow2Sn :
+  forall x n,
+    (2^n <= x < 2^(N.succ n))%N ->
+    N.testbit x n = true.
+Proof.
+  intros. assert (N.log2 x = n) by (apply N.log2_unique; lia).
+  rewrite <- H0. apply N.bit_log2.
+  assert (2^n <> 0)%N by (apply N.pow_nonzero; easy).
+  lia.
+Qed.
+
+Lemma negatem_Nlnot :
+  forall (n : nat) (x : N) i,
+    negatem n (N2fb x) i = N.testbit (N.lnot x (N.of_nat n)) (N.of_nat i).
+Proof.
+  intros. unfold negatem. rewrite N2fb_Ntestbit. symmetry.
+  bdestruct (i <? n). apply N.lnot_spec_low. lia.
+  apply N.lnot_spec_high. lia.
+Qed.
+
+Lemma negatem_arith :
+  forall n x,
+    x < 2^n ->
+    negatem n (nat2fb x) = nat2fb (2^n - 1 - x).
+Proof.
+  intros. unfold nat2fb. apply functional_extensionality; intro i.
+  rewrite negatem_Nlnot. rewrite N2fb_Ntestbit.
+  do 2 rewrite Nnat.Nat2N.inj_sub. rewrite Nofnat_pow. simpl.
+  bdestruct (x =? 0). subst. simpl. rewrite N.ones_equiv. rewrite N.pred_sub. rewrite N.sub_0_r. easy.
+  rewrite N.lnot_sub_low. rewrite N.ones_equiv. rewrite N.pred_sub. easy.
+  apply N.log2_lt_pow2. assert (0 < x) by lia. lia.
+  replace 2%N with (N.of_nat 2) by lia. rewrite <- Nofnat_pow. lia.
+Qed.
+
+
+(* Here, we define the addto / addto_n functions for angle rotation. *)
+Definition cut_n (f:nat -> bool) (n:nat) := fun i => if i <? n then f i else allfalse i.
+ 
+Definition fbrev' i n (f : nat -> bool) := fun (x : nat) => 
+            if (x <=? i) then f (n - 1 - x) else if (x <? n - 1 - i) 
+                         then f x else if (x <? n) then f (n - 1 - x) else f x.
+Definition fbrev {A} n (f : nat -> A) := fun (x : nat) => if (x <? n) then f (n - 1 - x) else f x.
+
+Lemma fbrev'_fbrev :
+  forall n f,
+    0 < n ->
+    fbrev n f = fbrev' ((n - 1) / 2) n f.
+Proof.
+  intros. unfold fbrev, fbrev'. apply functional_extensionality; intro.
+  assert ((n - 1) / 2 < n) by (apply Nat.div_lt_upper_bound; lia).
+  assert (2 * ((n - 1) / 2) <= n - 1) by (apply Nat.mul_div_le; easy).
+  assert (n - 1 - (n - 1) / 2 <= (n - 1) / 2 + 1).
+  { assert (n - 1 <= 2 * ((n - 1) / 2) + 1).
+    { assert (2 <> 0) by easy.
+      specialize (Nat.mul_succ_div_gt (n - 1) 2 H2) as G.
+      lia.
+    }
+    lia.
+  }
+  IfExpSimpl; easy.
+Qed.
+
+Lemma allfalse_0 : forall n, cut_n allfalse n = nat2fb 0.
+Proof.
+  intros. unfold nat2fb. simpl.
+  unfold cut_n.
+  apply functional_extensionality; intro.
+  bdestruct (x <? n).
+  easy. easy.
+Qed.
+
+Lemma f_num_aux_0: forall n f x, cut_n f n = nat2fb x 
+                -> f n = false -> cut_n f (S n) = nat2fb x.
+Proof.
+  intros.
+  rewrite <- H.
+  unfold cut_n.
+  apply functional_extensionality.
+  intros.
+  bdestruct (x0 <? n).
+  bdestruct (x0 <? S n).
+  easy.
+  lia.
+  bdestruct (x0 <? S n).
+  assert (x0 = n) by lia.
+  subst. rewrite H0. easy.
+  easy.
+Qed.
+
+Definition twoton_fun (n:nat) := fun i => if i <? n then false else if i=? n then true else false.
+
+
+Definition times_two_spec (f:nat -> bool) :=  fun i => if i =? 0 then false else f (i-1).
+
+(* Showing the times_two spec is correct. *)
+
+Lemma nat2fb_even_0:
+  forall x, nat2fb (2 * x) 0 = false.
+Proof.
+  intros.
+  unfold nat2fb.
+  rewrite Nat2N.inj_double.
+  unfold N.double.
+  destruct (N.of_nat x).
+  unfold N2fb,allfalse.
+  reflexivity.
+  unfold N2fb.
+  simpl.
+  reflexivity.
+Qed.
+
+Lemma pos2fb_times_two_eq:
+  forall p x, x <> 0 -> pos2fb p (x - 1) = pos2fb p~0 x.
+Proof.
+  intros.
+  induction p.
+  simpl.
+  assert ((fb_push false (fb_push true (pos2fb p))) x = (fb_push true (pos2fb p)) (x - 1)).
+  rewrite fb_push_right.
+  reflexivity. lia.
+  rewrite H0.
+  reflexivity.
+  simpl.
+  rewrite (fb_push_right x).
+  reflexivity. lia.
+  simpl.
+  rewrite (fb_push_right x).
+  reflexivity. lia.
+Qed.
+
+Lemma times_two_correct:
+   forall x, (times_two_spec (nat2fb x)) = (nat2fb (2*x)).
+Proof.
+  intros.
+  unfold times_two_spec.
+  apply functional_extensionality; intros.
+  unfold nat2fb.
+  bdestruct (x0 =? 0).
+  rewrite H.
+  specialize (nat2fb_even_0 x) as H3.
+  unfold nat2fb in H3.
+  rewrite H3.
+  reflexivity.
+  rewrite Nat2N.inj_double.
+  unfold N.double,N2fb.
+  destruct (N.of_nat x).
+  unfold allfalse.
+  reflexivity.
+  rewrite pos2fb_times_two_eq.
+  reflexivity. lia.
+Qed.
+
+
+Lemma f_twoton_eq : forall n, twoton_fun n = nat2fb (2^n).
+Proof.
+  intros.
+  induction n.
+  simpl.
+  unfold twoton_fun.
+  apply functional_extensionality.
+  intros. 
+  IfExpSimpl.
+  unfold fb_push. destruct x. easy. lia.
+  unfold fb_push. destruct x. lia. easy.
+  assert ((2 ^ S n) = 2 * (2^n)). simpl. lia.
+  rewrite H.
+  rewrite <- times_two_correct.
+  rewrite <- IHn.
+  unfold twoton_fun,times_two_spec.
+  apply functional_extensionality; intros.
+  bdestruct (x =? 0).
+  subst.
+  bdestruct (0 <? S n).
+  easy. lia.
+  bdestruct (x <? S n).
+  bdestruct (x - 1 <? n).
+  easy. lia.
+  bdestruct (x =? S n).
+  bdestruct (x - 1 <? n). lia.
+  bdestruct (x - 1 =? n). easy.
+  lia.
+  bdestruct (x-1<? n). easy.
+  bdestruct (x-1 =? n). lia.
+  easy.
+Qed.
+
+Local Transparent carry.
+
+Lemma carry_cut_n_false : forall i n f, carry false i (cut_n f n) (twoton_fun n) = false.
+Proof.
+  intros.
+  induction i.
+  simpl. easy.
+  simpl. rewrite IHi.
+  unfold cut_n,twoton_fun.
+  IfExpSimpl. btauto.
+  simpl.
+  btauto.
+  simpl. easy.
+Qed.
+
+Lemma carry_lt_same : forall m n f g h b, m < n -> (forall i, i < n -> f i = g i)
+                          -> carry b m f h = carry b m g h.
+Proof.
+ induction m; intros; simpl. easy.
+ rewrite H0. rewrite (IHm n) with (g:= g); try lia. easy.
+ easy. lia.
+Qed.
+
+Lemma carry_lt_same_1 : forall m n f g h h' b, m < n -> (forall i, i < n -> f i = g i)
+                 -> (forall i, i < n -> h i = h' i) -> carry b m f h = carry b m g h'.
+Proof.
+ induction m; intros; simpl. easy.
+ rewrite H1. rewrite H0. rewrite (IHm n) with (g:= g) (h' := h'); try lia. easy.
+ easy. easy. lia. lia.
+Qed.
+
+Local Opaque carry.
+
+Lemma sumfb_cut_n : forall n f, f n = true -> sumfb false (cut_n f n) (twoton_fun n)  = cut_n f (S n).
+Proof.
+  intros.
+  unfold sumfb.
+  apply functional_extensionality; intros.
+  rewrite carry_cut_n_false.
+  unfold cut_n, twoton_fun.
+  IfExpSimpl. btauto.
+  subst. rewrite H. simpl.  easy.
+  simpl. easy.
+Qed.
+
+Lemma f_num_aux_1: forall n f x, cut_n f n = nat2fb x -> f n = true 
+                  -> cut_n f (S n) = nat2fb (x + 2^n).
+Proof.
+  intros.
+  rewrite <- sumfb_correct_carry0.
+  rewrite <- H.
+  rewrite <- f_twoton_eq.
+  rewrite sumfb_cut_n.
+  easy. easy.
+Qed.
+
+Lemma f_num_0 : forall f n, (exists x, cut_n f n = nat2fb x).
+Proof.
+  intros.
+  induction n.
+  exists 0.
+  rewrite <- (allfalse_0 0).
+  unfold cut_n.
+  apply functional_extensionality.
+  intros.
+  bdestruct (x <? 0).
+  inv H. easy.
+  destruct (bool_dec (f n) true).
+  destruct IHn.
+  exists (x + 2^n).
+  rewrite (f_num_aux_1 n f x).
+  easy. easy. easy.
+  destruct IHn.
+  exists x. rewrite (f_num_aux_0 n f x).
+  easy. easy.
+  apply not_true_is_false in n0. easy.
+Qed.
+
+Lemma cut_n_1_1: forall (r:rz_val), r 0 = true -> cut_n r 1 = nat2fb 1.
+Proof.
+  intros. unfold cut_n.
+  apply functional_extensionality. intros.
+  bdestruct (x <? 1).
+  assert (x = 0) by lia. subst.
+  unfold nat2fb. simpl. rewrite H. easy.
+  unfold nat2fb. simpl. 
+  rewrite fb_push_right. easy. lia.
+Qed.
+
+Lemma cut_n_1_0: forall (r:rz_val), r 0 = false -> cut_n r 1 = nat2fb 0.
+Proof.
+  intros. unfold cut_n.
+  apply functional_extensionality. intros.
+  bdestruct (x <? 1).
+  assert (x = 0) by lia. subst.
+  unfold nat2fb. simpl. rewrite H. easy.
+  unfold nat2fb. simpl. easy.
+Qed.
+
+Lemma nat2fb_0: nat2fb 0 = allfalse.
+Proof.
+ unfold nat2fb. simpl. easy.
+Qed.
+
+Lemma pos2fb_no_zero : forall p, (exists i, pos2fb p i = true).
+Proof.
+  intros. induction p.
+  simpl. exists 0.
+  simpl. easy.
+  simpl. destruct IHp.
+  exists (S x).
+  simpl. easy. simpl.
+  exists 0. simpl. easy.
+Qed.
+
+Lemma cut_n_eq : forall n f, (forall i, i >= n -> f i = false) -> cut_n f n = f.
+Proof.
+ intros. unfold cut_n.
+ apply functional_extensionality; intro.
+ bdestruct (x <? n). easy. rewrite H. easy. lia. 
+Qed.
+
+
+
+Lemma nat2fb_bound : forall n x, x < 2^n -> (forall i, i >= n -> nat2fb x i = false).
+Proof.
+ intros. 
+ unfold nat2fb in *. 
+ assert ((N.of_nat x < (N.of_nat 2)^ (N.of_nat n))%N).
+ rewrite <- Nofnat_pow. lia.
+ apply N.mod_small in H1.
+ rewrite N2fb_Ntestbit.
+ rewrite <- H1.
+ apply N.mod_pow2_bits_high. lia.
+Qed.
+
+Lemma pos2fb_sem : forall x y, pos2fb x = pos2fb y -> x = y.
+Proof.
+ induction x; intros.
+ simpl in *.
+ destruct y. simpl in H.
+ assert (forall i, fb_push true (pos2fb x) i = fb_push true (pos2fb y) i).
+ intros. rewrite H. easy.
+ apply fb_push_same in H0. apply IHx in H0. subst. easy.
+ simpl in H.
+ assert (forall i, fb_push true (pos2fb x) i = fb_push false (pos2fb y) i).
+ intros. rewrite H. easy.
+ specialize (H0 0). simpl in H0. inv H0.
+ simpl in H.
+ assert (forall i, fb_push true (pos2fb x) i = fb_push true allfalse i).
+ intros. rewrite H. easy.
+ apply fb_push_same in H0.
+ specialize (pos2fb_no_zero x) as eq1.
+ destruct eq1. rewrite H0 in H1. unfold allfalse in H1. inv H1.
+ destruct y. simpl in *.
+ assert (forall i, fb_push false (pos2fb x) i = fb_push true (pos2fb y) i).
+ intros. rewrite H. easy.
+ specialize (H0 0). simpl in H0. inv H0.
+ simpl in *.
+ assert (forall i, fb_push false (pos2fb x) i = fb_push false (pos2fb y) i).
+ intros. rewrite H. easy.
+ apply fb_push_same in H0. apply IHx in H0. subst. easy.
+ simpl in *.
+ assert (forall i, fb_push false (pos2fb x) i = fb_push true allfalse i).
+ intros. rewrite H. easy.
+ specialize (H0 0). simpl in H0. inv H0.
+ destruct y. simpl in *.
+ assert (forall i, fb_push true allfalse i = fb_push true (pos2fb y) i).
+ intros. rewrite H. easy.
+ apply fb_push_same in H0. 
+ specialize (pos2fb_no_zero y) as eq1. destruct eq1.
+ rewrite <- H0 in H1. unfold allfalse in H1. inv H1.
+ simpl in *. 
+ assert (forall i, fb_push true allfalse i = fb_push false (pos2fb y) i).
+ intros. rewrite H. easy.
+ specialize (H0 0). simpl in H0. inv H0. easy.
+Qed.
+
+Lemma nat2fb_sem : forall x y, nat2fb x = nat2fb y -> x = y.
+Proof.
+  intros. unfold nat2fb,N2fb in H.
+  destruct (N.of_nat x) eqn:eq1.
+  destruct (N.of_nat y) eqn:eq2.
+  simpl in eq1. lia.
+  specialize (pos2fb_no_zero p) as eq3.
+  destruct eq3.
+  rewrite <- H in H0. unfold allfalse in H0. inv H0.
+  destruct (N.of_nat y) eqn:eq2.
+  specialize (pos2fb_no_zero p) as eq3.
+  destruct eq3.
+  rewrite H in H0. unfold allfalse in H0. inv H0.
+  apply pos2fb_sem in H. subst.
+  rewrite <- eq1 in eq2. lia.
+Qed.
+
+Lemma f_num_small : forall f n x, cut_n f n = nat2fb x -> x < 2^n.
+Proof.
+  induction n; intros. simpl in *.
+  assert (cut_n f 0 = allfalse).
+  unfold cut_n.
+  apply functional_extensionality.
+  intros. bdestruct (x0 <? 0). lia. easy.
+  rewrite H0 in H.
+  unfold nat2fb in H.
+  unfold N2fb in H.
+  destruct (N.of_nat x) eqn:eq1. lia.
+  specialize (pos2fb_no_zero p) as eq2.
+  destruct eq2. rewrite <- H in H1. unfold allfalse in H1.
+  inv H1.
+  specialize (f_num_0 f n) as eq1.
+  destruct eq1.
+  destruct (f n) eqn:eq2.
+  rewrite f_num_aux_1 with (x := x0) in H; try easy.
+  apply IHn in H0. simpl.
+  apply nat2fb_sem in H. subst. lia.
+  rewrite f_num_aux_0 with (x := x0) in H; try easy.
+  apply nat2fb_sem in H. subst.
+  apply IHn in H0. simpl. lia.
+Qed.
+
+Definition addto (r : nat -> bool) (n:nat) : nat -> bool := fun i => if i <? n 
+                    then (cut_n (fbrev n (sumfb false (cut_n (fbrev n r) n) (nat2fb 1))) n) i else r i.
+
+Definition addto_n (r:nat -> bool) n := fun i => if i <? n
+               then (cut_n (fbrev n (sumfb false (cut_n (fbrev n r) n) (negatem n (nat2fb 0)))) n) i else r i.
+
+Lemma addto_n_0 : forall r, addto_n r 0 = r.
+Proof.
+  intros.
+  unfold addto_n.
+  apply functional_extensionality.
+  intros.
+  IfExpSimpl. easy.
+Qed.
+
+Lemma addto_0 : forall r, addto r 0 = r.
+Proof.
+  intros.
+  unfold addto.
+  apply functional_extensionality.
+  intros.
+  IfExpSimpl. easy.
+Qed.
+
+Lemma cut_n_fbrev_flip : forall n f, cut_n (fbrev n f) n = fbrev n (cut_n f n).
+Proof.
+  intros.
+  unfold cut_n, fbrev.
+  apply functional_extensionality.
+  intros.
+  bdestruct (x <? n).
+  bdestruct (n - 1 - x <? n).
+  easy. lia. easy.
+Qed.
+
+Lemma cut_n_if_cut : forall n f g, cut_n (fun i => if i <? n then f i else g i) n = cut_n f n.
+Proof.
+  intros.
+  unfold cut_n.
+  apply functional_extensionality; intros.
+  bdestruct (x <? n).
+  easy. easy.
+Qed.
+
+Lemma fbrev_twice_same {A}: forall n f, @fbrev A n (fbrev n f) = f.
+Proof.
+  intros.
+  unfold fbrev.
+  apply functional_extensionality.
+  intros.
+  bdestruct (x <? n).
+  bdestruct (n - 1 - x <? n).
+  assert ((n - 1 - (n - 1 - x)) = x) by lia.
+  rewrite H1. easy.
+  lia. easy.
+Qed.
+
+Lemma cut_n_mod : forall n x, cut_n (nat2fb x) n = (nat2fb (x mod 2^n)).
+Proof.
+  intros.
+  bdestruct (x <? 2^n).
+  rewrite Nat.mod_small by lia.
+  unfold cut_n.
+  apply functional_extensionality; intros.
+  bdestruct (x0 <? n). easy.
+  specialize (nat2fb_bound n x H x0) as eq1.
+  rewrite eq1. easy. lia.
+  unfold cut_n.
+  apply functional_extensionality; intros.
+  bdestruct (x0 <? n).
+  unfold nat2fb.
+  rewrite N2fb_Ntestbit.
+  rewrite N2fb_Ntestbit.
+  rewrite <- N.mod_pow2_bits_low with (n := N.of_nat n).
+  rewrite Nofnat_mod.
+  rewrite Nofnat_pow. simpl. easy.
+  apply Nat.pow_nonzero. lia. lia.
+  assert (x mod 2 ^ n < 2^n).
+  apply Nat.mod_small_iff.
+  apply Nat.pow_nonzero. lia.
+  rewrite Nat.mod_mod. easy.
+  apply Nat.pow_nonzero. lia.  
+  specialize (nat2fb_bound n (x mod 2^n) H1 x0 H0) as eq1.
+  rewrite eq1. easy.
+Qed.
+
+Lemma add_to_r_same : forall q r, addto (addto_n r q) q = r.
+Proof.
+  intros.
+  destruct q eqn:eq1.
+  rewrite addto_n_0.
+  rewrite addto_0. easy.
+  unfold addto_n.
+  specialize (f_num_0 (fbrev (S n) r) (S n)) as eq2.
+  destruct eq2.
+  rewrite negatem_arith.
+  rewrite H.
+  rewrite sumfb_correct_carry0.
+  assert (1 < 2 ^ (S n)).
+  apply Nat.pow_gt_1. lia. lia.
+  assert (((2 ^ S n - 1 - 0)) = 2^ S n -1) by lia.
+  rewrite H1.
+  unfold addto.
+  rewrite (cut_n_fbrev_flip (S n) (fun i0 : nat =>
+                 if i0 <? S n
+                 then
+                  cut_n
+                    (fbrev (S n)
+                       (nat2fb
+                          (x + (2 ^ S n - 1))))
+                    (S n) i0
+                 else r i0)).
+  rewrite cut_n_if_cut.
+  rewrite (cut_n_fbrev_flip (S n)
+                      (nat2fb
+                         (x + (2 ^ S n - 1)))).
+  rewrite cut_n_mod.
+  rewrite <- cut_n_fbrev_flip.
+  rewrite fbrev_twice_same.
+  rewrite cut_n_mod.
+  rewrite Nat.mod_mod by lia.
+  rewrite sumfb_correct_carry0.
+  assert (((x + (2 ^ S n - 1)) mod 2 ^ S n + 1) = ((x + (2 ^ S n - 1)) mod 2 ^ S n + (1 mod 2^ S n))).
+  assert (1 mod 2^ S n = 1).
+  rewrite Nat.mod_small. easy. easy.
+  rewrite H2. easy.
+  rewrite H2.
+  rewrite cut_n_fbrev_flip.
+  rewrite cut_n_mod.
+  rewrite <- Nat.add_mod by lia.
+  assert ((x + (2 ^ S n - 1) + 1) = x + 2 ^ S n) by lia.
+  rewrite H3.
+  rewrite Nat.add_mod by lia.
+  rewrite Nat.mod_same by lia.
+  assert (x mod 2 ^ S n = x).
+  rewrite Nat.mod_small. easy.
+  apply (f_num_small (fbrev (S n) r)). easy.
+  rewrite H4.
+  rewrite plus_0_r.
+  rewrite H4.
+  rewrite <- H.
+  rewrite <- cut_n_fbrev_flip.
+  rewrite fbrev_twice_same.
+  apply functional_extensionality.
+  intros.
+  bdestruct (x0 <? S n).
+  unfold cut_n.
+  bdestruct (x0 <? S n).
+  easy. lia. easy.
+  specialize (Nat.pow_nonzero 2 (S n)) as eq2.
+  assert (2 <> 0) by lia. apply eq2 in H0. lia.
+Qed.
+
+Lemma add_to_same : forall q r, addto_n (addto r q) q = r.
+Proof.
+  intros.
+  destruct q eqn:eq1.
+  rewrite addto_n_0.
+  rewrite addto_0. easy.
+  unfold addto.
+  specialize (f_num_0 (fbrev (S n) r) (S n)) as eq2.
+  destruct eq2.
+  rewrite H.
+  rewrite sumfb_correct_carry0.
+  unfold addto_n.
+  assert (0 < 2^ (S n)).
+  specialize (Nat.pow_nonzero 2 (S n)) as eq2.
+  assert (2 <> 0) by lia. apply eq2 in H0. lia.
+  rewrite negatem_arith by lia.
+  rewrite (cut_n_fbrev_flip (S n) (fun i0 : nat =>
+                 if i0 <? S n
+                 then
+                  cut_n
+                    (fbrev (S n)
+                       (nat2fb (x + 1))) 
+                    (S n) i0
+                 else r i0)).
+  rewrite cut_n_if_cut.
+  rewrite (cut_n_fbrev_flip (S n)
+                      (nat2fb (x+1))).
+  rewrite cut_n_mod.
+  rewrite <- cut_n_fbrev_flip.
+  rewrite fbrev_twice_same.
+  rewrite cut_n_mod.
+  rewrite Nat.mod_mod by lia.
+  assert ((2 ^ S n - 1) = (2 ^ S n - 1) mod (2^ S n)).
+  rewrite Nat.mod_small by lia.
+  easy.
+  rewrite H1.
+  rewrite sumfb_correct_carry0.
+  rewrite cut_n_fbrev_flip.
+  rewrite cut_n_mod.
+  assert ((x + 1) mod 2 ^ S n + ((2 ^ S n - 1) mod 2 ^ S n - 0)
+           = ((x + 1) mod 2 ^ S n + ((2 ^ S n - 1) mod 2 ^ S n))) by lia.
+  rewrite H2.
+  rewrite <- Nat.add_mod by lia.
+  assert ((x + 1 + (2 ^ S n - 1))  = x + 2 ^ S n) by lia.
+  rewrite H3.
+  rewrite Nat.add_mod by lia.
+  rewrite Nat.mod_same by lia.
+  rewrite plus_0_r.
+  rewrite Nat.mod_mod by lia.
+  rewrite Nat.mod_small.
+  rewrite <- H.
+  rewrite cut_n_fbrev_flip.
+  rewrite fbrev_twice_same.
+  apply functional_extensionality.
+  intros.
+  bdestruct (x0 <? S n).
+  unfold cut_n.
+  bdestruct (x0 <? S n).
+  easy. lia. easy.
+  apply (f_num_small (fbrev (S n) r)). easy.
+Qed.
+
+
+Lemma posi_neq_f : forall (p p' : posi), p <> p' -> fst p <> fst p' \/ snd p <> snd p'.
+Proof.
+ intros. destruct p. destruct p'.
+ simpl in *.
+ bdestruct (v =? v0).
+ subst. right.
+ intros R. subst. contradiction.
+ bdestruct (n =? n0).
+ subst.
+ left.
+ intros R. subst. contradiction.
+ left. lia.
+Qed.
+
+Lemma posi_neq_b : forall (p p' : posi), fst p <> fst p' \/ snd p <> snd p' -> p <> p'.
+Proof.
+ intros. destruct p. destruct p'.
+ simpl in *.
+ intros R. inv R.
+ destruct H.
+ lia.
+ lia.
+Qed.
+
